many updates

experiments/coq-experiments/rbtnew/Analysis.py
@@ -26,15 +26,21 @@ def analyze(results: str, images: str):
     # colors = list(reversed(colors))
 
     strategies = [
-                    'BespokeGenerator',
-                    'TypeBasedGenerator',
-                    'ManualTypeBased2Generator',
-                    'CondEntropyInvariants2Generator',
-                    'ParentsCondEntropyInvariantsGenerator',
-                    'EntropyOnly2Generator',
-                    'NoRedRedGenerator',
-                    'TypeBasedDepth3Generator',
-                    'TypeBasedDepth4Generator',
+    # "BespokeGenerator",
+    "TypeBasedGenerator",
+    # "ManualTypeBased5Generator",
+    "ManualTypeBased5bGenerator",
+    # "atrained_Generator",
+    # "ctrained_Generator",
+    # "ftrained_Generator",
+    "fine_consider_1Generator",
+    "fine_ignore_1Generator",
+    "fine_consider_2Generator",
+    "fine_ignore_2Generator",
+    "uniformish_ignoreGenerator",
+    "uniformish_considerGenerator",
+    "uniform_considerGenerator",
+    "uniform_ignoreGenerator",
         ]
 
     for workload in ['RBT']:
