workloads/Coq/BST/Strategies/BespokeGenerator.v
@@ -19,11 +19,11 @@ Fixpoint gen_bst (s : nat) (lo hi : nat) : G Tree :=
                     ret (T l k v r))]
   end.
 
-Definition bespoke := gen_bst 5 0 40.
+Definition gSized := gen_bst 5 0 40.
 
 
 Definition test_prop_InsertValid   :=
-  forAll bespoke (fun (t: Tree)  =>
+  forAll gSized (fun (t: Tree)  =>
   forAll arbitrary (fun (k: nat)  =>
   forAll arbitrary (fun (v: nat) =>
   prop_InsertValid t k v)))
@@ -32,7 +32,7 @@ Definition test_prop_InsertValid   :=
 (*! QuickChick test_prop_InsertValid. *)
 
 Definition test_prop_DeleteValid   :=
-  forAll bespoke (fun (t: Tree)  =>
+  forAll gSized (fun (t: Tree)  =>
   forAll arbitrary (fun (k: nat) =>
   prop_DeleteValid t k))
 .
@@ -41,15 +41,15 @@ Definition test_prop_DeleteValid   :=
 
 
 Definition test_prop_UnionValid    :=
-  forAll bespoke (fun (t1: Tree)  =>
-  forAll bespoke (fun (t2: Tree) =>
+  forAll gSized (fun (t1: Tree)  =>
+  forAll gSized (fun (t2: Tree) =>
   prop_UnionValid t1 t2))
 .
 
 (*! QuickChick test_prop_UnionValid. *)
 
 Definition test_prop_InsertPost    :=
-  forAll bespoke (fun (t: Tree)  =>
+  forAll gSized (fun (t: Tree)  =>
   forAll arbitrary (fun (k: nat)  =>
   forAll arbitrary (fun (k': nat)  =>
   forAll arbitrary (fun (v: nat) =>
@@ -59,7 +59,7 @@ Definition test_prop_InsertPost    :=
 (*! QuickChick test_prop_InsertPost. *)
 
 Definition test_prop_DeletePost    :=
-  forAll bespoke (fun (t: Tree)  =>
+  forAll gSized (fun (t: Tree)  =>
   forAll arbitrary (fun (k: nat)  =>
   forAll arbitrary (fun (k': nat) =>
   prop_DeletePost t k k')))
@@ -68,8 +68,8 @@ Definition test_prop_DeletePost    :=
 (*! QuickChick test_prop_DeletePost. *)
 
 Definition test_prop_UnionPost   :=
-  forAll bespoke (fun (t: Tree)  =>
-  forAll bespoke (fun (t': Tree)  =>
+  forAll gSized (fun (t: Tree)  =>
+  forAll gSized (fun (t': Tree)  =>
   forAll arbitrary (fun (k: nat) =>
   prop_UnionPost t t' k)))
 .
@@ -77,7 +77,7 @@ Definition test_prop_UnionPost   :=
 (*! QuickChick test_prop_UnionPost. *)
 
 Definition test_prop_InsertModel   :=
-  forAll bespoke (fun (t: Tree)  =>
+  forAll gSized (fun (t: Tree)  =>
   forAll arbitrary (fun (k: nat)  =>
   forAll arbitrary (fun (v: nat) =>
   prop_InsertModel t k v)))
@@ -86,7 +86,7 @@ Definition test_prop_InsertModel   :=
 (*! QuickChick test_prop_InsertModel. *)
 
 Definition test_prop_DeleteModel   :=
-  forAll bespoke (fun (t: Tree)  =>
+  forAll gSized (fun (t: Tree)  =>
   forAll arbitrary (fun (k: nat) =>
   prop_DeleteModel t k))
 .
@@ -94,15 +94,15 @@ Definition test_prop_DeleteModel   :=
 (*! QuickChick test_prop_DeleteModel. *)
 
 Definition test_prop_UnionModel    :=
-  forAll bespoke (fun (t: Tree)  =>
-  forAll bespoke (fun (t': Tree) =>
+  forAll gSized (fun (t: Tree)  =>
+  forAll gSized (fun (t': Tree) =>
   prop_UnionModel t t'))
 .
 
 (*! QuickChick test_prop_UnionModel. *)
 
 Definition test_prop_InsertInsert    :=
-  forAll bespoke (fun (t: Tree)  =>
+  forAll gSized (fun (t: Tree)  =>
   forAll arbitrary (fun (k: nat)  =>
   forAll arbitrary (fun (k': nat)  =>
   forAll arbitrary (fun (v: nat)  =>
@@ -113,7 +113,7 @@ Definition test_prop_InsertInsert    :=
 (*! QuickChick test_prop_InsertInsert. *)
 
 Definition test_prop_InsertDelete    :=
-  forAll bespoke (fun (t: Tree)  =>
+  forAll gSized (fun (t: Tree)  =>
   forAll arbitrary (fun (k: nat)  =>
   forAll arbitrary (fun (k': nat)  =>
   forAll arbitrary (fun (v: nat) =>
@@ -123,8 +123,8 @@ Definition test_prop_InsertDelete    :=
 (*! QuickChick test_prop_InsertDelete. *)
 
 Definition test_prop_InsertUnion   :=
-  forAll bespoke (fun (t: Tree)  =>
-  forAll bespoke (fun (t': Tree)  =>
+  forAll gSized (fun (t: Tree)  =>
+  forAll gSized (fun (t': Tree)  =>
   forAll arbitrary (fun (k: nat)  =>
   forAll arbitrary (fun (v: nat) =>
   prop_InsertUnion t t' k v))))
@@ -133,7 +133,7 @@ Definition test_prop_InsertUnion   :=
 (*! QuickChick test_prop_InsertUnion. *)
 
 Definition test_prop_DeleteInsert    :=
-  forAll bespoke (fun (t: Tree)  =>
+  forAll gSized (fun (t: Tree)  =>
   forAll arbitrary (fun (k: nat)  =>
   forAll arbitrary (fun (k': nat)  =>
   forAll arbitrary (fun (v': nat) =>
@@ -143,7 +143,7 @@ Definition test_prop_DeleteInsert    :=
 (*! QuickChick test_prop_DeleteInsert. *)
 
 Definition test_prop_DeleteDelete    :=
-  forAll bespoke (fun (t: Tree)  =>
+  forAll gSized (fun (t: Tree)  =>
   forAll arbitrary (fun (k: nat)  =>
   forAll arbitrary (fun (k': nat) =>
   (prop_DeleteDelete t k k'))))
@@ -152,8 +152,8 @@ Definition test_prop_DeleteDelete    :=
 (*! QuickChick test_prop_DeleteDelete. *)
 
 Definition test_prop_DeleteUnion   :=
-  forAll bespoke (fun (t: Tree)  =>
-  forAll bespoke (fun (t': Tree)  =>
+  forAll gSized (fun (t: Tree)  =>
+  forAll gSized (fun (t': Tree)  =>
   forAll arbitrary (fun (k: nat) =>
   prop_DeleteUnion t t' k)))
 .
@@ -161,8 +161,8 @@ Definition test_prop_DeleteUnion   :=
 (*! QuickChick test_prop_DeleteUnion. *)
 
 Definition test_prop_UnionDeleteInsert   :=
-  forAll bespoke (fun (t :Tree)  =>
-  forAll bespoke (fun (t': Tree)  =>
+  forAll gSized (fun (t :Tree)  =>
+  forAll gSized (fun (t': Tree)  =>
   forAll arbitrary (fun (k: nat)  =>
   forAll arbitrary (fun (v: nat) =>
   (prop_UnionDeleteInsert t t' k v)))))
@@ -171,16 +171,16 @@ Definition test_prop_UnionDeleteInsert   :=
 (*! QuickChick test_prop_UnionDeleteInsert. *)
 
 Definition test_prop_UnionUnionIdem    :=
-  forAll bespoke (fun (t: Tree) =>
+  forAll gSized (fun (t: Tree) =>
   prop_UnionUnionIdem t)
 .
 
 (*! QuickChick test_prop_UnionUnionIdem. *)
 
 Definition test_prop_UnionUnionAssoc   :=
-  forAll bespoke (fun (t1: Tree)  =>
-  forAll bespoke (fun (t2: Tree)  =>
-  forAll bespoke (fun (t3: Tree) =>
+  forAll gSized (fun (t1: Tree)  =>
+  forAll gSized (fun (t2: Tree)  =>
+  forAll gSized (fun (t3: Tree) =>
   prop_UnionUnionAssoc t1 t2 t3)))
 .
 
