workloads/Coq/BST/oldstrats/ManualTypeBasedGenerator.v
@@ -1,0 +1,220 @@
+From QuickChick Require Import QuickChick. Import QcNotation.
+From Coq Require Import List. Import ListNotations.
+From Coq Require Import ZArith.
+From ExtLib Require Import Monad.
+Import MonadNotation.
+
+From BST Require Import Impl.
+From BST Require Import Spec.
+
+Definition manual_gen := 
+    fun s : nat =>
+    (let
+       fix arb_aux (size : nat) : G Tree :=
+         match size with
+         | 0 => returnGen E
+         | S size' =>
+             freq [ (1, returnGen E);
+             (1,
+             bindGen (arb_aux size')
+               (fun p0 : Tree =>
+                bindGen arbitrary
+                  (fun p1 : nat =>
+                   bindGen arbitrary
+                     (fun p2 : nat =>
+                      bindGen (arb_aux size')
+                        (fun p3 : Tree => returnGen (T p0 p1 p2 p3))))))]
+         end in
+     arb_aux) s.
+
+#[global]
+Instance genTree : GenSized (Tree) := 
+  {| arbitrarySized n := manual_gen n |}.
+
+Definition manual_shrink_tree := 
+    fun x : Tree =>
+    let
+      fix aux_shrink (x' : Tree) : list Tree :=
+        match x' with
+        | E => []
+        | T p0 p1 p2 p3 =>
+            ([p0] ++
+             map (fun shrunk : Tree => T shrunk p1 p2 p3) (aux_shrink p0) ++
+             []) ++
+            (map (fun shrunk : nat => T p0 shrunk p2 p3) (shrink p1) ++ []) ++
+            (map (fun shrunk : nat => T p0 p1 shrunk p3) (shrink p2) ++ []) ++
+            ([p3] ++
+             map (fun shrunk : Tree => T p0 p1 p2 shrunk) (aux_shrink p3) ++
+             []) ++ []
+        end in
+    aux_shrink x.
+
+
+#[global]
+Instance shrTree : Shrink (Tree) := 
+  {| shrink x := manual_shrink_tree x |}.
+
+Definition test_prop_InsertValid   :=
+  forAll arbitrary (fun (t: Tree)  =>
+  forAll arbitrary (fun (k: nat)  =>
+  forAll arbitrary (fun (v: nat) =>
+  prop_InsertValid t k v)))
+.
+
+(*! QuickChick test_prop_InsertValid. *)
+
+Definition test_prop_DeleteValid   :=
+  forAll arbitrary (fun (t: Tree)  =>
+  forAll arbitrary (fun (k: nat) =>
+  prop_DeleteValid t k))
+.
+
+(*! QuickChick test_prop_DeleteValid. *)
+
+
+Definition test_prop_UnionValid    :=
+  forAll arbitrary (fun (t1: Tree)  =>
+  forAll arbitrary (fun (t2: Tree) =>
+  prop_UnionValid t1 t2))
+.
+
+(*! QuickChick test_prop_UnionValid. *)
+
+Definition test_prop_InsertPost    :=
+  forAll arbitrary (fun (t: Tree)  =>
+  forAll arbitrary (fun (k: nat)  =>
+  forAll arbitrary (fun (k': nat)  =>
+  forAll arbitrary (fun (v: nat) =>
+  prop_InsertPost t k k' v))))
+.
+
+(*! QuickChick test_prop_InsertPost. *)
+
+Definition test_prop_DeletePost    :=
+  forAll arbitrary (fun (t: Tree)  =>
+  forAll arbitrary (fun (k: nat)  =>
+  forAll arbitrary (fun (k': nat) =>
+  prop_DeletePost t k k')))
+.
+
+(*! QuickChick test_prop_DeletePost. *)
+
+Definition test_prop_UnionPost   :=
+  forAll arbitrary (fun (t: Tree)  =>
+  forAll arbitrary (fun (t': Tree)  =>
+  forAll arbitrary (fun (k: nat) =>
+  prop_UnionPost t t' k)))
+.
+
+(*! QuickChick test_prop_UnionPost. *)
+
+Definition test_prop_InsertModel   :=
+  forAll arbitrary (fun (t: Tree)  =>
+  forAll arbitrary (fun (k: nat)  =>
+  forAll arbitrary (fun (v: nat) =>
+  prop_InsertModel t k v)))
+.
+
+(*! QuickChick test_prop_InsertModel. *)
+
+Definition test_prop_DeleteModel   :=
+  forAll arbitrary (fun (t: Tree)  =>
+  forAll arbitrary (fun (k: nat) =>
+  prop_DeleteModel t k))
+.
+
+(*! QuickChick test_prop_DeleteModel. *)
+
+Definition test_prop_UnionModel    :=
+  forAll arbitrary (fun (t: Tree)  =>
+  forAll arbitrary (fun (t': Tree) =>
+  prop_UnionModel t t'))
+.
+
+(*! QuickChick test_prop_UnionModel. *)
+
+Definition test_prop_InsertInsert    :=
+  forAll arbitrary (fun (t: Tree)  =>
+  forAll arbitrary (fun (k: nat)  =>
+  forAll arbitrary (fun (k': nat)  =>
+  forAll arbitrary (fun (v: nat)  =>
+  forAll arbitrary (fun (v': nat) =>
+  prop_InsertInsert t k k' v v')))))
+.
+
+(*! QuickChick test_prop_InsertInsert. *)
+
+Definition test_prop_InsertDelete    :=
+  forAll arbitrary (fun (t: Tree)  =>
+  forAll arbitrary (fun (k: nat)  =>
+  forAll arbitrary (fun (k': nat)  =>
+  forAll arbitrary (fun (v: nat) =>
+  prop_InsertDelete t k k' v))))
+.
+
+(*! QuickChick test_prop_InsertDelete. *)
+
+Definition test_prop_InsertUnion   :=
+  forAll arbitrary (fun (t: Tree)  =>
+  forAll arbitrary (fun (t': Tree)  =>
+  forAll arbitrary (fun (k: nat)  =>
+  forAll arbitrary (fun (v: nat) =>
+  prop_InsertUnion t t' k v))))
+.
+
+(*! QuickChick test_prop_InsertUnion. *)
+
+Definition test_prop_DeleteInsert    :=
+  forAll arbitrary (fun (t: Tree)  =>
+  forAll arbitrary (fun (k: nat)  =>
+  forAll arbitrary (fun (k': nat)  =>
+  forAll arbitrary (fun (v': nat) =>
+  prop_DeleteInsert t k k' v'))))
+.
+
+(*! QuickChick test_prop_DeleteInsert. *)
+
+Definition test_prop_DeleteDelete    :=
+  forAllShrink arbitrary shrink (fun (t: Tree)  =>
+  forAllShrink arbitrary shrink (fun (k: nat)  =>
+  forAllShrink arbitrary shrink (fun (k': nat) =>
+  whenFail' (fun tt => show (t, k, k', delete k t, delete k' t, delete k (delete k' t), delete k' (delete k t)))
+  (prop_DeleteDelete t k k'))))
+.
+
+(*! QuickChick test_prop_DeleteDelete. *)
+
+Definition test_prop_DeleteUnion   :=
+  forAll arbitrary (fun (t: Tree)  =>
+  forAll arbitrary (fun (t': Tree)  =>
+  forAll arbitrary (fun (k: nat) =>
+  prop_DeleteUnion t t' k)))
+.
+
+(*! QuickChick test_prop_DeleteUnion. *)
+
+Definition test_prop_UnionDeleteInsert   :=
+  forAll arbitrary (fun (t :Tree)  =>
+  forAll arbitrary (fun (t': Tree)  =>
+  forAll arbitrary (fun (k: nat)  =>
+  forAll arbitrary (fun (v: nat) =>
+  prop_UnionDeleteInsert t t' k v))))
+.
+
+(*! QuickChick test_prop_UnionDeleteInsert. *)
+
+Definition test_prop_UnionUnionIdem    :=
+  forAll arbitrary (fun (t: Tree) =>
+  prop_UnionUnionIdem t)
+.
+
+(*! QuickChick test_prop_UnionUnionIdem. *)
+
+Definition test_prop_UnionUnionAssoc   :=
+  forAll arbitrary (fun (t1: Tree)  =>
+  forAll arbitrary (fun (t2: Tree)  =>
+  forAll arbitrary (fun (t3: Tree) =>
+  prop_UnionUnionAssoc t1 t2 t3)))
+.
+
+(*! QuickChick test_prop_UnionUnionAssoc. *)
