workloads/Coq/STLC/Strategies/test.v
@@ -1,0 +1,66 @@
+From QuickChick Require Import QuickChick. Import QcNotation.
+
+From Coq Require Import Bool ZArith List. Import ListNotations.
+
+From ExtLib Require Import Monad.
+
+From ExtLib.Data.Monads Require Import OptionMonad.
+
+Import MonadNotation.
+
+
+
+From STLC Require Import Impl Spec.
+
+
+
+Derive (Arbitrary) for Typ.
+
+Derive (Arbitrary) for Expr.
+
+
+
+Definition gSized := arbitrary.
+
+
+
+Definition test_prop_SinglePreserve :=
+
+  forAll arbitrary (fun (e: Expr) =>
+
+    prop_SinglePreserve e).
+
+
+
+
+
+(*! QuickChick test_prop_SinglePreserve. *)
+
+
+
+Definition test_prop_MultiPreserve :=
+
+  forAll arbitrary (fun (e: Expr) =>
+
+    prop_MultiPreserve e).
+
+
+
+(*! QuickChick test_prop_MultiPreserve. *)
+            Fixpoint num_apps (e: Expr) : nat :=
+                match e with
+                | (Abs _ e) => num_apps e
+                | (App e1 e2) => 1 + num_apps e1 + num_apps e2
+                | _ => 0
+                end.
+    Definition collect {A : Type} `{_ : Show A} (f : Expr  -> A)  : Checker :=  
+        forAll gSized (fun (t : Expr) =>
+            if isJust (mt t) then
+                collect (append "valid " (show (f t))) true
+            else
+                collect (append "invalid " (show (f t))) true
+        ).
+        
+Extract Constant Test.defNumTests => "10000".
+QuickChick (collect sizeSTLC).
+QuickChick (collect num_apps).
