workloads/Coq/STLC/oldstrats/Manual2TypeBasedGenerator.v
@@ -1,0 +1,61 @@
+ 
+From QuickChick Require Import QuickChick. Import QcNotation.
+From Coq Require Import Bool ZArith List. Import ListNotations.
+From ExtLib Require Import Monad.
+From ExtLib.Data.Monads Require Import OptionMonad.
+Import MonadNotation.
+
+From STLC Require Import Impl Spec.
+
+Fixpoint manual_gen_typ (size : nat) : G Typ :=
+  match size with
+  | 0 => returnGen TBool
+  | S size' =>
+      freq [ (1, returnGen TBool);
+      (1,
+      bindGen (manual_gen_typ size')
+        (fun p0 : Typ =>
+         bindGen (manual_gen_typ size')
+           (fun p1 : Typ => returnGen (TFun p0 p1))))]
+  end.
+
+#[global]
+Instance genTyp : GenSized (Typ) := 
+  {| arbitrarySized n := manual_gen_typ n |}.
+
+Fixpoint manual_gen_expr (size : nat) : G Expr :=
+  match size with
+  | 0 =>
+      oneOf [bindGen arbitrary (fun p0 : nat => returnGen (Var p0));
+      bindGen arbitrary (fun p0 : bool => returnGen (Bool p0))]
+  | S size' =>
+      freq [ (1,
+      bindGen arbitrary (fun p0 : nat => returnGen (Var p0)));
+      (1, bindGen arbitrary (fun p0 : bool => returnGen (Bool p0)));
+      (1,
+      bindGen arbitrary
+        (fun p0 : Typ =>
+         bindGen (manual_gen_expr size')
+           (fun p1 : Expr => returnGen (Abs p0 p1))));
+      (1,
+      bindGen (manual_gen_expr size')
+        (fun p0 : Expr =>
+         bindGen (manual_gen_expr size')
+           (fun p1 : Expr => returnGen (App p0 p1))))]
+  end.
+
+#[global]
+Instance genExpr : GenSized (Expr) := 
+  {| arbitrarySized n := manual_gen_expr n |}.
+  
+Definition test_prop_SinglePreserve :=
+  forAll arbitrary (fun (e: Expr) =>
+    prop_SinglePreserve e).
+
+(*! QuickChick test_prop_SinglePreserve. *)
+  
+Definition test_prop_MultiPreserve :=
+  forAll arbitrary (fun (e: Expr) =>
+    prop_MultiPreserve e).
+  
+(*! QuickChick test_prop_MultiPreserve. *)
