workloads/Coq/STLC/oldstrats/ManualTypeBasedGenerator.v
@@ -1,0 +1,69 @@
+ 
+From QuickChick Require Import QuickChick. Import QcNotation.
+From Coq Require Import Bool ZArith List. Import ListNotations.
+From ExtLib Require Import Monad.
+From ExtLib.Data.Monads Require Import OptionMonad.
+Import MonadNotation.
+
+From STLC Require Import Impl Spec.
+
+Definition manual_gen_typ :=
+    fun s : nat =>
+    (let
+       fix arb_aux (size : nat) : G Typ :=
+         match size with
+         | 0 => returnGen TBool
+         | S size' =>
+             freq [ (1, returnGen TBool);
+             (1,
+             bindGen (arb_aux size')
+               (fun p0 : Typ =>
+                bindGen (arb_aux size')
+                  (fun p1 : Typ => returnGen (TFun p0 p1))))]
+         end in
+     arb_aux) s.
+
+#[global]
+Instance genTyp : GenSized (Typ) := 
+  {| arbitrarySized n := manual_gen_typ n |}.
+
+Definition manual_gen_expr :=
+  fun s : nat =>
+  (let
+     fix arb_aux (size : nat) : G Expr :=
+       match size with
+       | 0 =>
+           oneOf [bindGen arbitrary (fun p0 : nat => returnGen (Var p0));
+           bindGen arbitrary (fun p0 : bool => returnGen (Bool p0))]
+       | S size' =>
+           freq [ (1,
+           bindGen arbitrary (fun p0 : nat => returnGen (Var p0)));
+           (1, bindGen arbitrary (fun p0 : bool => returnGen (Bool p0)));
+           (1,
+           bindGen arbitrary
+             (fun p0 : Typ =>
+              bindGen (arb_aux size')
+                (fun p1 : Expr => returnGen (Abs p0 p1))));
+           (1,
+           bindGen (arb_aux size')
+             (fun p0 : Expr =>
+              bindGen (arb_aux size')
+                (fun p1 : Expr => returnGen (App p0 p1))))]
+       end in
+   arb_aux) s.
+
+#[global]
+Instance genExpr : GenSized (Expr) := 
+  {| arbitrarySized n := manual_gen_expr n |}.
+  
+Definition test_prop_SinglePreserve :=
+  forAll arbitrary (fun (e: Expr) =>
+    prop_SinglePreserve e).
+
+(*! QuickChick test_prop_SinglePreserve. *)
+  
+Definition test_prop_MultiPreserve :=
+  forAll arbitrary (fun (e: Expr) =>
+    prop_MultiPreserve e).
+  
+(*! QuickChick test_prop_MultiPreserve. *)
